Added more of the spine of the proof of the forward simulation. The bisimulation relation is still the naive one, but even the proof of this naive part is... tricky.

Bisimulation.v
@@ -7,8 +7,11 @@ Require Import Util.
 Require Import Translation.
 
 
- Inductive related : (term * bool) -> (term * bool) -> Prop :=
-  | related_base : forall e thread base buf_size, related (e, thread) (translate e thread base buf_size, thread).
+Inductive related : (term * bool) -> (term * bool) -> Prop :=
+(*  | related_reflexive : forall e thread, related (e, thread) (e, thread)*)
+  | related_translate : forall e thread base buf_size, related (e, thread) (translate e thread base buf_size, thread).
+ 
+
 
 
 Definition related_terms (TSO_program : TSO.program) (SC_program : SC.program) (base : nat) : Prop :=
@@ -81,8 +84,66 @@ Definition related_program (p : TSO_machine) (q : SC_machine) (f : nat -> nat) (
   related_terms TSO_program SC_program B /\
   related_memory TSO_memory SC_memory B f.
 
+Fact contexts_respect_bisimilarity : forall E B s2 buffer f true e event e' mem mem' m t0 l t1,
+  related (s2, false) (t0, false) ->
+  related_memory mem m B f ->
+  step e event e' ->
+  TSO.memstep mem (true, event) mem' ->
+  related (con_subst E e, true) (t1, true) ->
+  (forall re : term,
+  related (e, true) (re, true) ->
+  exists q' : SC_machine,
+  related_program (buffer, nil, e', s2, mem') q' f B /\
+  SC_program_steps (l, re, t0, while tru (SPECIAL B [num 0]::= ZERO), m) q') ->
+  exists q' : SC_machine,
+  (related_program (buffer, nil, con_subst E e', s2, mem') q' f B /\
+  SC_program_steps (l, t1, t0, while tru (SPECIAL B [num 0]::= ZERO), m) q').
+Proof. intros. generalize dependent t1. induction E; intros; simpl in *.
+  + apply H4. auto.
+  + assert (exists q' : SC_machine,
+          related_program
+            (buffer, nil, con_subst E e', s2, mem') q'
+            f B /\
+          SC_program_steps
+            (l, translate (con_subst E e) true B buffer, t0,
+            while tru (SPECIAL B [num 0]::= ZERO), m)
+            q'). apply IHE. apply related_translate. destruct H5. destruct H5. destruct x. destruct p. destruct p. destruct p. destruct H5. simpl in *. destruct H7. destruct H7. simpl in *. inversion H3. inversion H7. subst. refine (ex_intro _ (l0, translate (app (con_subst E e') t) true B buffer, t3, t2, m0) _). split.
+    ++ unfold related_program. simpl. split.
+      +++ intros. contradiction H10. auto.
+      +++ split.
+        ++++ unfold related_terms. simpl in *. split.
+          - admit.
+          - split.
+            -- admit.
+            -- admit.
+        ++++ admit.
+    ++ simpl. admit.
+  + admit.
+  + admit.
+  + admit.
+  + admit.
+  + admit.
+  + admit.
+  + admit.
+  + admit.
+  + admit.
+  + admit.
+  + admit.
+  + admit.
+  + admit.
+  + admit.
+  + admit.
+  + admit.
+  + admit.
+  + admit.
+  + admit.
+  + admit.
+  + admit.
+Admitted.
+
+
 Theorem forward_bisimulation : forall p p' q f B,
-  TSO.pstep p p' -> related_program p q f B -> (exists q', related_program p' q' f B /\ psteps q q').
+  TSO.pstep p p' -> related_program p q f B -> (exists q', related_program p' q' f B /\ SC_program_steps q q').
   Proof. intros. inversion H; subst.
     + destruct q. destruct p. repeat (destruct p). destruct m. destruct mem. destruct mem'. repeat (destruct p0). repeat (destruct p). destruct H0. simpl in *. destruct H4. destruct H4. destruct H6. simpl in *. subst. assert (l = translate_arrays (xs ++ (size, init) :: nil) buffer). apply H0. intros C. symmetry in C. contradiction app_cons_not_nil with (x:=xs) (a:=(size, init)) (y:=nil). subst. remember (translate_arrays xs buffer, t1, t0, while tru (SPECIAL (length xs) [num 0]::= ZERO)) as answer_p. unfold related_memory in H5. simpl in *. destruct H5. destruct H7. destruct H7. remember (update_mapping (length xs) x size m, allocate x (x + size - 1) init g) as answer_m. refine (ex_intro _ (answer_p, answer_m) _); subst. admit.
     + destruct H0. simpl in *. destruct H3. destruct H3. destruct q. destruct p. destruct p. destruct p. simpl in *. clear H0. destruct H5. subst. generalize dependent t1. induction H1; intros; subst.
