SC.v
@@ -15,30 +15,30 @@ Definition update_global (val : nat * nat) (g : global_store) : global_store :=
 Definition update_mapping (location : nat) (base : nat) (size : nat) (g : mapping) : mapping :=
 (fun n => if Nat.eqb n location then Some (base, size) else g n).
 
-Inductive memstep : memory_model -> mem_event -> memory_model -> Prop :=
-  | ST_tau_step : forall mem, memstep mem Tau mem
+Inductive memory_step : memory_model -> mem_event -> memory_model -> Prop :=
+  | ST_tau_step : forall mem, memory_step mem Tau mem
   | ST_read :  forall global value location offset mapping base size,
                mapping location = Some (base, size) ->
                offset < size ->
                global (base + offset) = Some value ->
-               memstep (mapping, global) (Read location offset value) (mapping, global)
+               memory_step (mapping, global) (Read location offset value) (mapping, global)
   | ST_write : forall global global' offset value location mapping base size,
                mapping location = Some (base, size) ->
                offset < size ->
                global' = update_global (base + offset, value) global ->
-               memstep (mapping, global) (Write location offset value) (mapping, global')
+               memory_step (mapping, global) (Write location offset value) (mapping, global')
   | ST_allocate_array : forall global global' init location size mapping base mapping',
                (forall n, base <= n < base + size -> global n = None) ->
                mapping location = None ->
                mapping' = update_mapping location base size mapping ->
                global' = allocate base (base + size - 1) init global ->
-               memstep (mapping, global) (Allocate location size init) (mapping', global')
+               memory_step (mapping, global) (Allocate location size init) (mapping', global')
   | ST_reference : forall global location base size mapping,
                mapping location = Some (base, size) ->
-               memstep (mapping, global) (Reference location base) (mapping, global)
+               memory_step (mapping, global) (Reference location base) (mapping, global)
   | ST_cast : forall global location mapping base size,
                mapping location = Some (base, size) ->
-               memstep (mapping, global) (Cast base location) (mapping, global).
+               memory_step (mapping, global) (Cast base location) (mapping, global).
 
 (* A program is a 4-tuple (init, s1, s2, s3)
   2. init : (list (nat * (list nat))) denoting array variables with respective inital values,
@@ -54,58 +54,46 @@ Inductive pstep : SC_machine -> SC_machine -> Prop :=
   | ST_init_allocate_array : forall xs s1 s2 s3 mem mem' size init,
                       size > 0 ->
                       length init <= size ->
-                      memstep mem (Allocate (length xs) size init) mem' ->
+                      memory_step mem (Allocate (length xs) size init) mem' ->
                       pstep ((xs ++ ((size, init) :: nil), s1, s2, s3), mem)
                             ((xs, s1, s2, s3), mem')
   | ST_synchronize1 : forall s1 event s1' mem mem' s2 s3,
                       step s1 event s1' ->
-                      memstep mem event mem' ->
+                      memory_step mem event mem' ->
                       pstep ((nil, s1, s2, s3), mem)
                             ((nil, s1', s2, s3), mem')
   | ST_synchronize2 : forall s1 event s2' mem mem' s2 s3,
                       step s2 event s2' ->
-                      memstep mem event mem' ->
+                      memory_step mem event mem' ->
                       pstep ((nil, s1, s2, s3), mem)
                             ((nil, s1, s2', s3), mem')
   | ST_synchronize3 : forall s1 event s3' mem mem' s2 s3,
                       step s3 event s3' ->
-                      memstep mem event mem' ->
+                      memory_step mem event mem' ->
                       pstep ((nil, s1, s2, s3), mem)
                             ((nil, s1, s2, s3'), mem').
 
-Inductive psteps : SC_machine -> SC_machine -> Prop :=
-  | psteps_reflexive : forall p, psteps p p
-  | psteps_transitive : forall p q r, pstep p q -> psteps q r -> psteps p r.
+Inductive SC_program_steps : SC_machine -> SC_machine -> Prop :=
+  | SC_program_steps_reflexive : forall p, SC_program_steps p p
+  | SC_program_steps_transitive : forall p q r, pstep p q -> SC_program_steps q r -> SC_program_steps p r.
 
-(*Fact psteps_inj_1 : forall p q, psteps p q -> steps (snd (fst (fst (fst p)))) (snd (fst (fst (fst q)))).
-  Proof. intros. induction H.
-    + apply steps_reflexive.
-    + repeat (destruct p). repeat (destruct q). repeat (destruct r). simpl in *. simpl.
-      repeat (destruct p0). simpl. repeat (destruct p). simpl in *. inversion H; subst; auto.
-      apply steps_transitive with (event:=event) (q:=t7). auto. auto.
-  Qed.
+Inductive SC_thread_steps : (term * memory_model) -> (term * memory_model) -> Prop :=
+  | SC_thread_steps_reflexive : forall t, SC_thread_steps t t
+  | SC_thread_steps_transitive : forall e e' e'' m m' m'' event, memory_step m event m' ->
+      (step e event e' \/ e = e') -> SC_thread_steps (e', m') (e'', m'') ->
+      SC_thread_steps (e, m) (e'', m'').
 
-Fact psteps_inj_2 : forall p q, psteps p q -> steps (snd (fst (fst p))) (snd (fst (fst q))).
-  Proof. intros. induction H.
-    + apply steps_reflexive.
-    + repeat (destruct p). repeat (destruct q). repeat (destruct r). simpl in *. simpl.
-      repeat (destruct p0). simpl. repeat (destruct p). simpl in *. inversion H; subst; auto.
-      apply steps_transitive with (event:=event) (q:=t6). auto. auto.
-  Qed.
-
-Fact psteps_inj_3 : forall p q, psteps p q -> steps (snd (fst p)) (snd (fst q)).
-  Proof. intros. induction H.
-    + apply steps_reflexive.
-    + repeat (destruct p). repeat (destruct q). repeat (destruct r). simpl in *. simpl.
-      repeat (destruct p0). simpl. repeat (destruct p). simpl in *. inversion H; subst; auto.
-      apply steps_transitive with (event:=event) (q:=t5). auto. auto.
-  Qed.
-
-Fact psteps_transports : forall e e' E, steps e e' -> steps (subst E e) (subst E e').
-  Proof. intros. induction H.
-    + apply steps_reflexive.
-    + assert (step (subst E p) event (subst E q)).
-      {apply step_context. auto. }
-      apply steps_transitive with (event:=event) (q:=subst E q). auto. auto.
-  Qed.
-*)
+Fact SC_program_steps_to_SC_thread_steps : forall t t',
+(SC_program_steps t t' ->
+(SC_thread_steps (snd (fst (fst (fst t))), snd t) (snd (fst (fst (fst t'))), snd t') /\ 
+SC_thread_steps (snd (fst (fst t)), snd t) (snd (fst (fst t')), snd t') /\ 
+SC_thread_steps (snd (fst t), snd t) (snd (fst t'), snd t'))).
+  Proof. intros. induction H. 
+      ++ split. apply SC_thread_steps_reflexive. split. apply SC_thread_steps_reflexive. apply SC_thread_steps_reflexive.
+      ++ destruct IHSC_program_steps. destruct H2. repeat (destruct p). destruct q. repeat (destruct p). destruct r. repeat (destruct p). simpl in *. inversion H; subst; clear H.
+        +++ split. apply SC_thread_steps_transitive with (e':=t4) (event:=(Allocate (length l0) size init)) (m':=m0). auto. right. auto. auto. split. apply SC_thread_steps_transitive with (e':=t3) (event:=(Allocate (length l0) size init)) (m':=m0). auto. right. auto. auto. apply SC_thread_steps_transitive with (e':=t2) (event:=(Allocate (length l0) size init)) (m':=m0). auto. right. auto. auto.
+        +++ split. apply SC_thread_steps_transitive with (event:=event) (e':=t4) (m':=m0). auto. left. auto.
+auto. split. apply SC_thread_steps_transitive with (e':=t3) (event:=event) (m':=m0). auto. right. auto. auto.  apply SC_thread_steps_transitive with (e':=t2) (event:=event) (m':=m0). auto. right. auto. auto.
+        +++ split. apply SC_thread_steps_transitive with (e':=t4) (event:=event) (m':=m0). auto. right. auto. auto. split.  apply SC_thread_steps_transitive with (e':=t3) (event:=event) (m':=m0). auto. left. auto. auto.  apply SC_thread_steps_transitive with (e':=t2) (event:=event) (m':=m0). auto. right. auto. auto.
+        +++ split. apply SC_thread_steps_transitive with (e':=t4) (event:=event) (m':=m0). auto. right. auto. auto. split. apply SC_thread_steps_transitive with (e':=t3) (event:=event) (m':=m0). auto. right. auto. auto.  apply SC_thread_steps_transitive with (e':=t2) (event:=event) (m':=m0). auto. left. auto. auto.
+Qed.
